verified expr translation from L10 to L20

From10To20/Translate.v
@@ -1,5 +1,8 @@
-From Coq Require Import String ZArith.
-From Vyper Require Import Config.
+From Coq Require Import String ZArith Eqdep_dec.
+
+From Coq Require PropExtensionality.
+
+From Vyper Require Import Config Calldag L10.Base.
 From Vyper Require L10.AST L20.AST L10.Interpret L20.Interpret.
 
 Section Translate.
@@ -42,9 +45,9 @@ Fixpoint translate_small_stmt (ss: L10.AST.small_stmt)
 : L20.AST.stmt
 := match ss with
    | L10.AST.Pass => L20.AST.SmallStmt L20.AST.Pass
-   | L10.AST.Break    => L20.AST.SmallStmt (L20.AST.Abort (L10.Interpret.AbortBreak))
-   | L10.AST.Continue => L20.AST.SmallStmt (L20.AST.Abort (L10.Interpret.AbortContinue))
-   | L10.AST.Revert   => L20.AST.SmallStmt (L20.AST.Abort (L10.Interpret.AbortRevert))
+   | L10.AST.Break    => L20.AST.SmallStmt (L20.AST.Abort (AbortBreak))
+   | L10.AST.Continue => L20.AST.SmallStmt (L20.AST.Abort (AbortContinue))
+   | L10.AST.Revert   => L20.AST.SmallStmt (L20.AST.Abort (AbortRevert))
    | L10.AST.Return (Some result) => L20.AST.SmallStmt (L20.AST.Return (translate_expr result))
    | L10.AST.Return None => L20.AST.SmallStmt (L20.AST.Return (L20.AST.Const zero256))
    | L10.AST.Raise error => L20.AST.SmallStmt (L20.AST.Raise (translate_expr error))
@@ -253,10 +256,10 @@ Qed.
 (* The callsets of statement lists behave normally ASSUMING that each statement behaves normally.
    We'll get rid of this assumption later.
  *)
-Lemma callset_translate_stmt_list_aux {C: VyperConfig}
-                                      (is_private_call: string -> bool)
-                                      (l: list L10.AST.stmt)
-                                      (x: string)
+Local Lemma callset_translate_stmt_list_aux {C: VyperConfig}
+                                            (is_private_call: string -> bool)
+                                            (l: list L10.AST.stmt)
+                                            (x: string)
                  (Ok: let _ := string_set_impl in
                       List.Forall
                         (fun s : L10.AST.stmt =>
@@ -378,27 +381,27 @@ Qed.
 
 (*************************************************************************************************)
 
-Lemma translate_calldag_helper {C: VyperConfig}
-                               (cd: L10.Interpret.calldag):
+Local Lemma translate_calldag_helper {C: VyperConfig}
+                                     (cd: L10.Descend.calldag):
   let is_private_call (name: string)
-   := match L10.Interpret.cd_declmap cd name with
+   := match cd_declmap cd name with
       | Some _ => true
       | _ => false
       end 
   in forall name: string,
        match
-          match L10.Interpret.cd_declmap cd name with
+          match cd_declmap cd name with
           | Some f => Some (translate_decl is_private_call f)
           | None => None
           end
        with
        | Some decl =>
-           match L10.Interpret.cd_depthmap cd name with
+           match cd_depthmap cd name with
            | Some x =>
                let _ := string_set_impl in
                FSet.for_all (Callset.decl_callset decl)
                  (fun callee : string =>
-                  match L10.Interpret.cd_depthmap cd callee with
+                  match cd_depthmap cd callee with
                   | Some y => y <? x
                   | None => false
                   end) = true
@@ -408,42 +411,501 @@ Lemma translate_calldag_helper {C: VyperConfig}
        end.
 Proof.
 intros is_private_call name.
-assert (D := L10.Interpret.cd_depthmap_ok cd name).
+assert (D := cd_depthmap_ok cd name).
 cbn.
-remember (L10.Interpret.cd_declmap cd name) as maybe_f. destruct maybe_f. 2:easy.
-destruct (L10.Interpret.cd_depthmap cd name). 2:easy.
+remember (cd_declmap cd name) as maybe_f. destruct maybe_f. 2:easy.
+destruct (cd_depthmap cd name). 2:easy.
 rewrite FSet.for_all_ok in *. intros x H.
 rewrite callset_translate_decl in H.
 apply Bool.andb_true_iff in H.
 assert (Q := D x (proj1 H)). clear D.
-destruct (L10.Interpret.cd_depthmap cd x). 2:easy.
+destruct (cd_depthmap cd x). 2:easy.
 destruct n; rewrite Nat.ltb_lt in Q. { now apply Nat.nlt_0_r in Q. }
 rewrite Nat.leb_le.
 apply Nat.lt_succ_r. exact Q.
 Qed.
 
 
-(* XXX This is inefficient since functions are translated at each lookup.
+(* This is inefficient since functions are translated at each lookup.
    It's better to rebuild the calldag.
  *)
-Definition translate_calldag {C: VyperConfig} (cd: L10.Interpret.calldag)
+Definition translate_calldag {C: VyperConfig} (cd: L10.Descend.calldag)
+: L20.Descend.calldag
 := let is_private_call (name: string)
-   := match L10.Interpret.cd_declmap cd name with
+   := match cd_declmap cd name with
       | Some _ => true
       | _ => false
       end
-   in {| L20.Interpret.cd_declmap (name: string) :=
-              match L10.Interpret.cd_declmap cd name with
+   in {| cd_declmap (name: string) :=
+              match cd_declmap cd name with
               | Some f => Some (translate_decl is_private_call f)
               | None => None
               end
-       ; L20.Interpret.cd_depthmap := L10.Interpret.cd_depthmap cd
-       ; L20.Interpret.cd_depthmap_ok := translate_calldag_helper cd
+       ; cd_depthmap := cd_depthmap cd
+       ; cd_depthmap_ok := translate_calldag_helper cd
       |}.
 
 (***************************************************************************************************)
 
+Section FunCtx.
+  Context {C: VyperConfig}
+          {bound: nat}
+          {cd: L10.Descend.calldag}
+          (fc: fun_ctx cd bound)
+          {cd2: L20.Descend.calldag}
+          (ok: cd2 = translate_calldag cd).
+
+  Local Lemma translate_fun_ctx_depthmap_helper (name: string):
+    cd_depthmap cd2 name
+     =
+    cd_depthmap cd name.
+  Proof.
+  subst. trivial.
+  Qed.
+
+  Local Lemma translate_fun_ctx_fun_decl_helper:
+    cd_declmap cd2 (fun_name fc) <> None.
+  Proof.
+  intro E.
+  assert (Ok := fun_decl_ok fc).
+  subst cd2. cbn in E. rewrite Ok in E. discriminate.
+  Qed.
+
+  Definition cached_translated_decl
+  := match cd_declmap cd2 (fun_name fc)
+     as d' return _ = d' -> _
+     with
+     | Some f => fun _ => f
+     | None => fun E =>
+          False_rect _ (translate_fun_ctx_fun_decl_helper E)
+     end eq_refl.
+
+  Local Lemma translate_fun_ctx_decl_ok:
+    cd_declmap cd2 (fun_name fc) 
+     =
+    Some cached_translated_decl.
+  Proof.
+  assert (D := fun_decl_ok fc).
+  unfold cached_translated_decl.
+  remember translate_fun_ctx_fun_decl_helper as foo. clear Heqfoo. revert foo.
+  destruct (cd_declmap cd2 (fun_name fc)). { trivial. }
+  intro. contradiction.
+  Qed.
+
+  Definition translate_fun_ctx
+  : fun_ctx cd2 bound
+  := let name := fun_name fc in
+     {| fun_name := name
+      ; fun_depth := fun_depth fc
+      ; fun_depth_ok :=
+          eq_trans (translate_fun_ctx_depthmap_helper name)
+                   (fun_depth_ok fc)
+      ; fun_decl := cached_translated_decl
+      ; fun_decl_ok := translate_fun_ctx_decl_ok
+      ; fun_bound_ok := fun_bound_ok fc
+     |}.
+
+End FunCtx.
+(***************************************************************************************************)
+
+Lemma interpret_translated_expr {C: VyperConfig}
+                                {bigger_call_depth_bound smaller_call_depth_bound: nat}
+                                (Ebound: bigger_call_depth_bound = S smaller_call_depth_bound)
+                                {cd: L10.Descend.calldag}
+                                (builtins: string -> option builtin)
+                                (fc: fun_ctx cd bigger_call_depth_bound)
+                                {cd2: L20.Descend.calldag}
+                                (ok: cd2 = translate_calldag cd)
+                                {do_call_10: forall
+                                      (fc': fun_ctx cd smaller_call_depth_bound)
+                                      (world: world_state)
+                                      (arg_values: list uint256),
+                                    world_state * expr_result uint256}
+                                {do_call_20: forall
+                                      (fc': fun_ctx cd2 smaller_call_depth_bound)
+                                      (world: world_state)
+                                      (arg_values: list uint256),
+                                    world_state * expr_result uint256}
+                                (DoCallOk: forall fc' world arg_values,
+                                             do_call_20 (translate_fun_ctx fc' ok) world arg_values
+                                              =
+                                             do_call_10 fc' world arg_values)
+                                (world: world_state)
+                                (loc: string_map uint256)
+                                {e10: L10.AST.expr}
+                                {e20: L20.AST.expr}
+                                (ExprOk: e20 = let is_private_call := fun name: string =>
+                                                  match cd_declmap cd name with
+                                                  | Some _ => true
+                                                  | _ => false
+                                                  end
+                                               in translate_expr is_private_call e10)
+                                (CallOk20: let _ := string_set_impl in 
+                                   FSet.is_subset (L20.Callset.expr_callset e20)
+                                                  (L20.Callset.decl_callset
+                                                     (fun_decl
+                                                       (translate_fun_ctx fc ok)))
+                                   = true)
+                                (CallOk10: let _ := string_set_impl in 
+                                   FSet.is_subset (L10.Callset.expr_callset e10)
+                                                  (L10.Callset.decl_callset
+                                                    (fun_decl fc))
+                                   = true):
+   L20.Expr.interpret_expr Ebound (translate_fun_ctx fc ok) do_call_20 builtins
+                                world loc e20 CallOk20
+    =
+   L10.Expr.interpret_expr Ebound fc do_call_10 builtins
+                                world loc e10 CallOk10.
+Proof.
+revert e20 ExprOk CallOk20 world loc. induction e10 using L10.AST.expr_ind'; intros.
+{ (* Const *) now subst. }
+{ (* LocalVar *) now subst. }
+{ (* StorageVar *) now subst. }
+{ (* UnOp *)
+  subst. cbn.
+  rewrite (IHe10 (L10.Callset.callset_descend_unop eq_refl CallOk10)); trivial.
+}
+{ (* BinOp *)
+  subst. cbn.
+  rewrite (IHe10_1 (L10.Callset.callset_descend_binop_left eq_refl CallOk10)) by trivial.
+  destruct (L10.Expr.interpret_expr eq_refl fc do_call_10 builtins world loc e10_1
+             (L10.Callset.callset_descend_binop_left eq_refl CallOk10)) as (world_a, result_a).
+  destruct result_a. 2:{ trivial. }
+  rewrite (IHe10_2 (L10.Callset.callset_descend_binop_right eq_refl CallOk10)); trivial.
+}
+{ (* IfThenElse *)
+  subst. cbn.
+  rewrite (IHe10_1 (L10.Callset.callset_descend_if_cond eq_refl CallOk10)) by trivial.
+  destruct (L10.Expr.interpret_expr eq_refl fc do_call_10 builtins world loc e10_1
+             (L10.Callset.callset_descend_if_cond eq_refl CallOk10)) as (world_cond, result_cond).
+  destruct result_cond. 2:{ trivial. }
+  destruct ((Z_of_uint256 value =? 0)%Z).
+  { (* else *) rewrite (IHe10_3 (L10.Callset.callset_descend_if_else eq_refl CallOk10)); trivial. }
+  (* then *)   rewrite (IHe10_2 (L10.Callset.callset_descend_if_then eq_refl CallOk10)); trivial.
+}
+{ (* LogicalAnd *)
+  subst. cbn.
+  rewrite (IHe10_1 (L10.Callset.callset_descend_and_left eq_refl CallOk10)) by trivial.
+  destruct (L10.Expr.interpret_expr eq_refl fc do_call_10 builtins world loc e10_1
+             (L10.Callset.callset_descend_and_left eq_refl CallOk10)) as (world_a, result_a).
+  destruct result_a. 2:{ trivial. }
+  destruct ((Z_of_uint256 value =? 0)%Z). { trivial. }
+  rewrite (IHe10_2 (L10.Callset.callset_descend_and_right eq_refl CallOk10)); trivial.
+}
+{ (* LogicalOr *)
+  subst. cbn.
+  rewrite (IHe10_1 (L10.Callset.callset_descend_or_left eq_refl CallOk10)) by trivial.
+  destruct (L10.Expr.interpret_expr eq_refl fc do_call_10 builtins world loc e10_1
+             (L10.Callset.callset_descend_or_left eq_refl CallOk10)) as (world_a, result_a).
+  destruct result_a. 2:{ trivial. }
+  destruct ((Z_of_uint256 value =? 0)%Z). 2:{ trivial. }
+  rewrite (IHe10_2 (L10.Callset.callset_descend_or_right eq_refl CallOk10)); trivial.
+}
+(* call *)
+subst. cbn.
+cbn in CallOk20.
+remember (cd_declmap cd name) as d.
+destruct d; cbn;
+  remember (fix interpret_expr_list 
+                        (w: world_state) (loc: string_map uint256) 
+                        (exprs : list L20.AST.expr)
+                        (CallOk : FSet.is_subset (Callset.expr_list_callset exprs)
+                                    (L20.Callset.decl_callset (cached_translated_decl fc eq_refl))
+                                  = true)
+                        := _)
+    as interpret_expr_list_20;
+  remember (fix translate_expr_list (l: list L10.AST.expr): list L20.AST.expr := _)
+    as translate_expr_list;
+  remember (fix interpret_expr_list
+                        (w: world_state) (loc: string_map uint256) 
+                        (exprs : list L10.AST.expr)
+                        (CallOk : FSet.is_subset (L10.Callset.expr_list_callset exprs)
+                                    (L10.Callset.decl_callset
+                                       (fun_decl fc)) =
+                                  true)
+                        := _)
+    as interpret_expr_list_10.
+{ (* PrivateCall *)
+  assert (L: interpret_expr_list_20 world loc (translate_expr_list args)
+               (L20.Callset.callset_descend_args eq_refl CallOk20)
+              =
+             interpret_expr_list_10 world loc args 
+               (L10.Callset.callset_descend_args eq_refl CallOk10)).
+  {
+    remember (L20.Callset.callset_descend_args eq_refl CallOk20) as CallsOk20.
+    remember (L10.Callset.callset_descend_args eq_refl CallOk10) as CallsOk10.
+    clear CallOk10 HeqCallsOk10 CallOk20 HeqCallsOk20.
+    revert world loc. induction args. { now subst. }
+    intros. cbn in *.
+    assert (CallsOk10' := CallsOk10).
+    rewrite FSet.union_subset_and in CallsOk10'.
+    rewrite Bool.andb_true_iff in CallsOk10'.
+    destruct CallsOk10' as (HeadCallOk, TailCallsOk).
+    subst. cbn.
+    rewrite (List.Forall_inv H HeadCallOk) by trivial.
+    match goal with
+    |- (let (_, _) := ?l in _) = let (_, _) := ?r in _ =>
+       remember l as lhs_head_result;
+       remember r as rhs_head_result
+    end.
+    assert (R: lhs_head_result = rhs_head_result).
+    { subst. f_equal. apply Eqdep_dec.eq_proofs_unicity. decide equality. }
+    rewrite<- R.
+    clear Heqlhs_head_result Heqrhs_head_result R rhs_head_result.
+    destruct lhs_head_result as (world', result_h).
+    destruct result_h. 2:{ trivial. }
+    now rewrite (IHargs (List.Forall_inv_tail H)
+                        (L20.Callset.callset_descend_tail eq_refl CallsOk20)
+                        (L10.Callset.callset_descend_tail eq_refl CallsOk10) world' loc).
+  }
+  rewrite L.
+  clear L Heqinterpret_expr_list_10 Heqinterpret_expr_list_20 H.
+  destruct (interpret_expr_list_10 world loc args (L10.Callset.callset_descend_args eq_refl CallOk10))
+    as (world', result_args).
+  destruct result_args. 2:{ trivial. }
+  match goal with
+  |- _ = match ?x with Some _ => _ | None => _ end =>
+          remember x as maybe_ctx10
+  end.
+  clear interpret_expr_list_10 interpret_expr_list_20 world.
+  assert (D: L20.Descend.fun_ctx_descend (translate_fun_ctx fc eq_refl) CallOk20 eq_refl eq_refl
+              =
+             match maybe_ctx10 with
+             | Some ctx => Some (translate_fun_ctx ctx eq_refl)
+             | None => None
+             end).
+  {
+    (* This follows fun_ctx_descend_irrel. *)
+    unfold L10.Descend.fun_ctx_descend in Heqmaybe_ctx10.
+    unfold L20.Descend.fun_ctx_descend.
+    assert (InnerOk: forall (d1: L10.AST.decl)
+                            (Edecl1: cd_declmap cd name = Some d1)
+                            (d2: L20.AST.decl)
+                            (Edecl2: cd_declmap (translate_calldag cd) name = Some d2),
+                   L20.Descend.fun_ctx_descend_inner (translate_fun_ctx fc eq_refl) CallOk20 
+                                                     eq_refl eq_refl Edecl2
+                    =
+                   match L10.Descend.fun_ctx_descend_inner fc CallOk10 eq_refl eq_refl Edecl1 with
+                   | Some ctx10 => Some (translate_fun_ctx ctx10 eq_refl)
+                   | None => None
+                   end).
+    {
+      intros.
+      unfold L10.Descend.fun_ctx_descend_inner.
+      unfold L20.Descend.fun_ctx_descend_inner.
+      remember (fun (depth: nat) (Edepth: cd_depthmap (translate_calldag cd) name = Some depth) =>
+          Some
+            {|
+            fun_name := name;
+            fun_depth := depth;
+            fun_depth_ok := Edepth;
+            fun_decl := d2;
+            fun_decl_ok := Edecl2;
+            fun_bound_ok := L20.Descend.call_descend'
+                              (translate_fun_ctx fc eq_refl) CallOk20 eq_refl eq_refl
+                              Edecl2 Edepth |})
+        as some_branch_l.
+      remember (fun (Edepth: cd_depthmap (translate_calldag cd) name = None) =>
+        False_rect (option (fun_ctx (translate_calldag cd) smaller_call_depth_bound))
+          (Descend.fun_ctx_descend_helper Edecl2 Edepth))
+        as none_branch_l.
+      remember (fun (depth: nat) (Edepth: cd_depthmap cd name = Some depth) =>
+        Some
+          {|
+          fun_name := name;
+          fun_depth := depth;
+          fun_depth_ok := Edepth;
+          fun_decl := d1;
+          fun_decl_ok := Edecl1;
+          fun_bound_ok := L10.Descend.call_descend' fc CallOk10 eq_refl eq_refl Edecl1 Edepth |})
+        as some_branch_r.
+      remember (fun Edepth : cd_depthmap cd name = None =>
+                  False_rect (option (fun_ctx cd smaller_call_depth_bound))
+                             (L10.Descend.fun_ctx_descend_helper Edecl1 Edepth))
+        as none_branch_r.
+      assert (NoneOkL: forall (Edepth: cd_depthmap (translate_calldag cd) name = None),
+                         none_branch_l Edepth = None).
+      { intro. exfalso. exact (Descend.fun_ctx_descend_helper Edecl2 Edepth). }
+      assert (NoneOkR: forall (Edepth: cd_depthmap cd name = None),
+                         none_branch_r Edepth = None).
+      { intro. exfalso. exact (L10.Descend.fun_ctx_descend_helper Edecl1 Edepth). }
+      clear Heqnone_branch_l Heqnone_branch_r.
+      revert none_branch_l none_branch_r NoneOkL NoneOkR.
+      assert (SomeBranchOk: forall (depth: nat)
+                                   (Edepth1: cd_depthmap cd name = Some depth)
+                                   (Edepth2: cd_depthmap (translate_calldag cd) name = Some depth),
+                     some_branch_l depth Edepth2 
+                      =
+                     match some_branch_r depth Edepth1 with
+                     | Some ctx10 => Some (translate_fun_ctx ctx10 eq_refl)
+                     | None => None
+                     end).
+      {
+        intros. subst. unfold translate_fun_ctx. cbn.
+        f_equal.
+        assert (D: d2 = cached_translated_decl
+                {|
+                fun_name := name;
+                fun_depth := depth;
+                fun_depth_ok := Edepth1;
+                fun_decl := d1;
+                fun_decl_ok := Edecl1;
+                fun_bound_ok := L10.Descend.call_descend' fc CallOk10 eq_refl eq_refl Edecl1 Edepth1 |}
+                eq_refl).
+        {
+          unfold cached_translated_decl. cbn.
+          remember (translate_fun_ctx_fun_decl_helper _ eq_refl) as Bad. clear HeqBad.
+          cbn in Bad. revert Bad.
+          rewrite Edecl1.
+          intro Bad. clear Bad.
+          unfold translate_calldag in Edecl2. cbn in Edecl2. rewrite Edecl1 in Edecl2.
+          symmetry in Edecl2. inversion Edecl2. trivial.
+        }
+        subst. f_equal; apply PropExtensionality.proof_irrelevance.
+      } (* SomeBranchOk *)
+      clear Heqsome_branch_l Heqsome_branch_r Heqmaybe_ctx10 translate_expr_list Heqtranslate_expr_list
+            CallOk10 CallOk20 Edecl1 Edecl2 d1 d2 maybe_ctx10 world' loc args value DoCallOk
+            do_call_10 do_call_20.
+      assert (R: cd_depthmap (translate_calldag cd) name = cd_depthmap cd name). { trivial. }
+      revert some_branch_l some_branch_r SomeBranchOk.
+      rewrite R. clear R.
+      destruct (cd_depthmap cd name); intros. { apply SomeBranchOk. }
+      rewrite (NoneOkL eq_refl).
+      rewrite (NoneOkR eq_refl).
+      trivial.
+    } (* InnerOk *)
+    remember L20.Descend.fun_ctx_descend_inner as inner20. clear Heqinner20.
+    remember L10.Descend.fun_ctx_descend_inner as inner10. clear Heqinner10.
+    subst.
+    revert inner10 inner20 InnerOk.
+    remember (cd_declmap cd name) as maybe_d1.
+    remember (cd_declmap (translate_calldag cd) name) as maybe_d2.
+    destruct maybe_d1; destruct maybe_d2; intros. 4:{ trivial. }
+    { apply InnerOk. }
+    1-2: exfalso; clear inner10 inner20 InnerOk.
+    1-2: unfold translate_calldag in Heqmaybe_d2; cbn in Heqmaybe_d2; 
+           rewrite<- Heqmaybe_d1 in Heqmaybe_d2; discriminate.
+  } (* D *)
+  rewrite D.
+  assert (DNone := L10.Descend.fun_ctx_descend_none fc CallOk10 eq_refl eq_refl).
+  destruct maybe_ctx10.
+  { apply DoCallOk. }
+  exfalso. rewrite<- Heqmaybe_ctx10 in DNone.
+  rewrite<- Heqd in DNone.
+  assert (Bad: Some d = None) by tauto.
+  discriminate.
+}
+(* BuiltinCall *)
+  assert (L: interpret_expr_list_20 world loc (translate_expr_list args)
+               (L20.Callset.callset_descend_builtin_args eq_refl CallOk20)
+              =
+             interpret_expr_list_10 world loc args 
+               (L10.Callset.callset_descend_args eq_refl CallOk10)).
+  {
+    remember (L20.Callset.callset_descend_builtin_args eq_refl CallOk20) as CallsOk20.
+    remember (L10.Callset.callset_descend_args eq_refl CallOk10) as CallsOk10.
+    clear CallOk10 HeqCallsOk10 CallOk20 HeqCallsOk20.
+    revert world loc. induction args. { now subst. }
+    intros. cbn in *.
+    assert (CallsOk10' := CallsOk10).
+    rewrite FSet.union_subset_and in CallsOk10'.
+    rewrite Bool.andb_true_iff in CallsOk10'.
+    destruct CallsOk10' as (HeadCallOk, TailCallsOk).
+    subst. cbn.
+    rewrite (List.Forall_inv H HeadCallOk) by trivial.
+    match goal with
+    |- (let (_, _) := ?l in _) = let (_, _) := ?r in _ =>
+       remember l as lhs_head_result;
+       remember r as rhs_head_result
+    end.
+    assert (R: lhs_head_result = rhs_head_result).
+    { subst. f_equal. apply Eqdep_dec.eq_proofs_unicity. decide equality. }
+    rewrite<- R.
+    clear Heqlhs_head_result Heqrhs_head_result R rhs_head_result.
+    destruct lhs_head_result as (world', result_h).
+    destruct result_h. 2:{ trivial. }
+    now rewrite (IHargs (List.Forall_inv_tail H)
+                        (L20.Callset.callset_descend_tail eq_refl CallsOk20)
+                        (L10.Callset.callset_descend_tail eq_refl CallsOk10) world' loc).
+  }
+  rewrite L.
+  clear L Heqinterpret_expr_list_10 Heqinterpret_expr_list_20 H.
+  destruct (interpret_expr_list_10 world loc args (L10.Callset.callset_descend_args eq_refl CallOk10))
+    as (world', result_args).
+  destruct result_args. 2:{ trivial. }
+  assert (DNone := L10.Descend.fun_ctx_descend_none fc CallOk10 eq_refl eq_refl).
+  symmetry in Heqd.
+  apply DNone in Heqd.
+  rewrite Heqd.
+  trivial.
+Qed.
+
 (*
+Theorem interpret_translated_call {C: VyperConfig}
+                                  (builtins: string -> option L10.Interpret.builtin)
+                                  {cd: L10.Interpret.calldag}
+                                  {call_depth_bound: nat}
+                                  (fc: L10.Interpret.fun_ctx cd call_depth_bound)
+                                  {cd2: L20.Interpret.calldag}
+                                  (ok: cd2 = translate_calldag cd)
+                                  (world: world_state)
+                                  (arg_values: list uint256):
+  L20.Interpret.interpret_call builtins (translate_fun_ctx fc ok) world arg_values
+   =
+  L10.Interpret.interpret_call builtins fc world arg_values.
+Proof.
+induction call_depth_bound.
+{ exfalso. exact (Nat.nlt_0_r _ (L10.Interpret.fun_bound_ok _ _ fc)). }
+pose (is_private_call := fun name: string =>
+          match L10.Interpret.cd_declmap _ _ cd name with
+          | Some _ => true
+          | _ => false
+          end).
+assert(F: L20.Interpret.fun_decl _ _ (translate_fun_ctx fc ok)
+           = 
+          translate_decl is_private_call (L10.Interpret.fun_decl _ _ fc)).
+{
+  clear IHcall_depth_bound.
+  unfold translate_fun_ctx in *. cbn in *.
+  unfold cached_translated_decl in *.
+  remember (translate_fun_ctx_fun_decl_helper fc ok) as foo. clear Heqfoo.
+  remember (Interpret.cd_declmap cd2 (L10.Interpret.fun_name cd (S call_depth_bound) fc)) as d.
+  destruct d. 2:{ contradiction. }
+  subst. cbn in Heqd.
+  remember (L10.Interpret.cd_declmap L10.AST.decl L10.Callset.decl_callset cd
+                                     (L10.Interpret.fun_name cd (S call_depth_bound) fc)) as x.
+  destruct x. 2:{ discriminate. }
+  inversion Heqd. unfold is_private_call.
+  f_equal. inversion Heqx.
+  assert (D := L10.Interpret.fun_decl_ok _ _ fc).
+  rewrite D in *. inversion H1. (* XXX *)
+  trivial.
+}
+unfold L20.Interpret.interpret_call.
+unfold L10.Interpret.interpret_call.
+rewrite F.
+
+
+
+
+
+
+  intro H. clear H.
+  
+  
+  
+remember  as d10.
+
+
+unfold translate_fun_ctx. unfold cached_translated_decl.
+remember (L10.Interpret.fun_name _ _ fc) as fun_name.
+
+unfold translate_fun_ctx.
+
+
+
+
+
 Theorem translate_ok {C: VyperConfig}
                      (builtins: string -> option L10.Interpret.builtin)
                      (cd: L10.Interpret.calldag)
@@ -454,5 +916,11 @@ Theorem translate_ok {C: VyperConfig}
    =
   L10.Interpret.interpret builtins cd fun_name world arg_values.
 Proof.
-unfold L10.Interpret.interpret.
-unfold L20.Interpret.interpret. *)
+unfold L10.Interpret.interpret. unfold L20.Interpret.interpret.
+remember (L10.Interpret.cd_declmap cd fun_name) as d. 
+unfold translate_calldag.
+unfold L20.Interpret.make_fun_ctx_and_bound. cbn.
+revert translate_dag_helper.
+destruct d.
+*)
+
